further relaxed limit typing and ext to discard lim_min

theories/typing.v
@@ -267,11 +267,11 @@ https://www.w3.org/TR/wasm-core-2/appendix/properties.html#store-validity
 **)
 Section Store_validity.
 
-(* exactly limits_extension;
+(* limits_extension without lim_min condition (like Wasm 1.0);
   though this corresponds to Wasm 1.0 typing on limits,
   so does the extension definition so this should be intentional *)
 Definition limits_typing (l1 l2 : limits) : bool :=
-  (l1.(lim_min) <= l2.(lim_min)) &&
+  (* (l1.(lim_min) <= l2.(lim_min)) && *)
   (l1.(lim_max) == l2.(lim_max)).
 
 Definition funci_agree (fs : seq function_closure) (n : funcaddr) (f : function_type) : bool :=
